proof/gate.ec
@@ -3,6 +3,7 @@ require import Int.
 require import Map.
 require import Pair.
 require import Bool.
+require import Array.
 
 require import Dkc.
 require import GarbleTools.
@@ -30,7 +31,7 @@ clone Scheme as Gate with
 
   op eval(f:funct, i:input) = evalGate f i,
 
-  op _garble(x:random, f:funct) =
+  op garble(x:random, f:funct) =
     (garbleGate x f 0 1 2, x, tt),
 
   op encrypt(k:keyInput, i:input) =
@@ -50,20 +51,54 @@ lemma inverse :
   forall (f : funct) , functCorrect f =>
   forall (x : random) , randomCorrect f x =>
   forall (i : input) , inputCorrect f i =>
-    let (g, ki, ko) = _garble x f in
+    let (g, ki, ko) = garble x f in
     eval f i = decrypt ko (evalG g (encrypt ki i))
 proof.
   intros f fC x xC i iC.
   cut main : (
-    let (g, ki, ko) = _garble x f in
+    let (g, ki, ko) = garble x f in
     evalG g (encrypt ki i) = getTok x 2 (eval f i)
   ).
-    delta _garble decrypt eval evalG encrypt.
+    delta garble decrypt eval evalG encrypt.
     simplify.
   apply (inverse_base i 2 1 1 0 1 2 f x _ _ _ _ _ _ _);trivial.
-  cut main2 : (let (g, ki, ko) = _garble x f in
+  cut main2 : (let (g, ki, ko) = garble x f in
     eval f i = decrypt ko (getTok x 2 (eval f i)));trivial.
 save.
 
+module RandGate : Rand_t = {
+  fun genT() : bool*bool = {
+    var t0 : bool;
+    var t1 : bool;
+    t0 = $Dbool.dbool;
+    t1 = $Dbool.dbool;
+    return (t0, t1);
+  }
+    
+  fun genR(t:bool*bool) : random = {
+    var r : tokens;
+    var r0f : token;
+    var r0t : token;
+    var r1f : token;
+    var r1t : token;
+    var r2f : token;
+    var r2t : token;
+    var t0,t1 : bool*bool = t;
+    r0f = $Dkc.genRandKeyLast(t0);
+    r1t = $Dkc.genRandKeyLast(!t0);
+    r1f = $Dkc.genRandKeyLast(t1);
+    r1t = $Dkc.genRandKeyLast(!t1);
+    r2f = $Dkc.genRandKeyLast(false);
+    r2t = $Dkc.genRandKeyLast(true);
+    r = Array.empty:::(r0f, r0t):::(r1f, r1t):::(r2f, r2t);
+    return r;
+  }
 
-  
+  fun gen() : random = {
+    var r : tokens;
+    var t : bool*bool;
+    t := genT();
+    r := genR(t);
+    return r;
+  }
+}.
