proof/proofGate.ec
@@ -12,272 +12,8 @@ require import Gate.
 require import GarbleTools.
 require AdvGate.
 
-
-lemma map : (forall (m:('a, 'b) map, x:'a, y:'b), proj m.[x <- y].[x] = y).
-
-op opQuery : Gate.query.
-op opB : bool.
-module Adv : Gate.Adv = {
-  fun gen_query() : Gate.query = {return opQuery;}
-  fun get_challenge(answer:Gate.answer) : bool = {return opB;}
-}.
-
-lemma realEq :
-  forall (Adv <: Gate.Adv),
-    equiv [
-      Dkc.Game(Dkc.Dkc, AdvGate.Adv(Adv)).work ~
-        Gate.Game(Gate.PrvInd, Adv).main :
-      (Dkc.Dkc.b{1}) /\ (AdvGate.Adv.l{1}=0)
-      ==> res{1} = res{2}
-    ]
-proof.
-admit.
-save.
-
-
-lemma middleEq :
-      forall (Adv <: Gate.Adv),
-        equiv [
-          Dkc.Game(Dkc.Dkc, AdvGate.Adv(Adv)).work ~
-            Dkc.Game(Dkc.Dkc, AdvGate.Adv(Adv)).work :
-          (!Dkc.Dkc.b{1}) /\ (AdvGate.Adv.l{1}=0) /\
-          (Dkc.Dkc.b{2}) /\ (AdvGate.Adv.l{1}=1)
-          ==> !res{1} = res{2}
-        ]
-proof.
-  intros Adv.
-  fun.
-  call (AdvGate.Adv.l{1}=0/\AdvGate.Adv.l{2}=1) (res{1}=res{2}).
-    fun.
-    call (answer{1}=answer{2}) (res{1}=res{2});[admit(*ADV rule*)|intros ch1 ch2].
-    wp.
-    app 1 2 : (AdvGate.Adv.input{1}=AdvGate.Adv.input{2}/\AdvGate.Adv.g{1}=AdvGate.Adv.g{2}/\AdvGate.Adv.l{1}=0/\AdvGate.Adv.l{2}=1).
-    rcondf {2} 1;[intros &m;skip;trivial|].
-    rcondt {1} 1;[intros &m;skip;trivial|].
-    rcondt {2} 1;[intros &m;skip;trivial|].
-    call (true) (AdvGate.Adv.input{1}=AdvGate.Adv.input{2}/\AdvGate.Adv.g{1}=AdvGate.Adv.g{2}).
-
-
-cut intro : (
-          let preG_1 = AdvGate.Adv.preG{m1} in
-          let preG_2 = AdvGate.Adv.preG{m2} in
-          let g_1 = AdvGate.Adv.g{m1} in
-          let g_2 = AdvGate.Adv.g{m2} in
-          let fc = AdvGate.Adv.fc{m2} in
-          let tau = AdvGate.Adv.tau{m2} in
-          let x = AdvGate.Adv.x{m2} in
-          let vis1 = (AdvGate.get AdvGate.Adv.xc{m2} 0)^^(proj AdvGate.Adv.t{m2}.[0]) in
-equiv [AdvGate.Adv(Adv).computeG1 ~ AdvGate.Adv(Adv).computeG2 : (*&t1=&1/\&t2=&2*) true ==> AdvGate.Adv.input {1} =
-  AdvGate.Adv.input {2} /\
-  AdvGate.Adv.g {1} = AdvGate.Adv.g {2}]
-);[|apply intro].
-      
-      intros preG1 preG2 g_1 g_2 fc tau x vis1.
-      fun.
-      wp.
-      call (AdvGate.Adv.fc{1}=AdvGate.Adv.fc{2}/\AdvGate.Adv.xc{1}=AdvGate.Adv.xc{2}/\
-        AdvGate.Adv.x{1}=AdvGate.Adv.x{2}/\ AdvGate.Adv.t{1}=AdvGate.Adv.t{2}/\
-        AdvGate.Adv.g{1}=AdvGate.Adv.g{2}/\AdvGate.Adv.input{1}=AdvGate.Adv.input{2}/\(          if vis1 = tau then
-            forall b, proj preG1.[(!vis1, b)] = proj preG2.[(!vis1, b)]
-          else
-            proj preG1.[(vis1, !tau)] = proj preG2.[(!vis1, !tau)])
-        )
-        (AdvGate.Adv.input{1}=AdvGate.Adv.input{2}/\(
-          if vis1 = tau then
-            (forall b, proj g_1.[(!vis1, b)] = proj g_2.[(!vis1, b)]) /\
-            proj g_1.[(vis1,   !tau)] = AdvGate.enc x preG1 fc vis1 (!tau)
-          else
-            proj g_1.[(vis1, !tau)] = proj g_2.[(!vis1, !tau)] /\
-            proj g_1.[(vis1,  tau)] = AdvGate.enc x preG1 fc vis1 tau /\
-            proj g_2.[(tau,  true)] = AdvGate.enc x preG2 fc tau true /\
-            proj g_2.[(tau,  false)] = AdvGate.enc x preG2 fc tau false
-        )).
-  (*
-          let g_1 = AdvGate.Adv.g{2} in
-          let g_2 = AdvGate.Adv.g{2} in
-          let tau = AdvGate.Adv.tau{2} in
-          let xc = AdvGate.Adv.xc{2} in
-          let x = AdvGate.Adv.x{2} in
-          let t = AdvGate.Adv.t{2} in
-          let x1 = get xc 0 in
-          let x2 = get xc 1 in
-          let t2 = proj t.[1] in
-          let val0 = Gate.eval fc (!x1, false) in
-          let val1 = Gate.eval fc (!x1, true) in
-          let vis1 = x1^^(proj t.[0]) in
- *)
-        fun.
-        wp.
-        skip.
-        intros &1 &2 h.
-        split.
-        trivial.
-
-        elim h; clear h; intros h1 h;
-        elim h; clear h; intros h2 h;
-        elim h; clear h; intros h3 h;
-        elim h; clear h; intros h4 h;
-        elim h; clear h; intros h5 h;
-        elim h; clear h; intros h6.
-
-        cut lem1 : (forall b1 b2, proj (Map.__get g_1 (b1, b2)) = AdvGate.enc AdvGate.Adv.x{1} preG1 AdvGate.Adv.fc{1} b1 b2). (*TODO*) admit.
-        cut lem2 : (forall b1 b2, proj (Map.__get g_2 (b1, b2)) = AdvGate.enc AdvGate.Adv.x{2} preG1 AdvGate.Adv.fc{2} b1 b2). (*TODO*) admit.
-
-        case (vis1 = tau).
-        intros hvt h.
-
-
-
-        split.
-        intros b.
-        rewrite (lem1 (!vis1) b).
-        rewrite (lem2 (!vis1) b).
-        delta AdvGate.enc.
-        simplify.
-        rewrite (_ : proj preG1.[(!vis1,  b)] = proj preG2.[(!vis1, b)]);[apply (h b)|trivial].
-        rewrite (lem1 vis1 (!tau)).
-        rewrite h1.
-        rewrite h3.
-        delta x fc.
-        trivial.
-
-
-          admit. (*TODO:*)
-        split.
-          admit. (*TODO:*)
-        admit.
-        intros hvt.
-        split.
-          admit. (*TODO:*)
-        split.
-          admit. (*TODO:*)
-        admit.
-      intros _ _.
-        
-        trivial.
-      intros _ _.
-      app 11 8 : true.
-        call true true.
-        fun.
-        call true true.
-        fun.
-        wp.
-    intros _ _.
-    rcondf {1} 1;[intros &m;skip;trivial|].
-    rcondf {1} 1;[intros &m;skip;trivial|].
-    rcondf {2} 1;[intros &m;skip;trivial|].
-    skip.
-    intros &1 &2 h.
-    split.
-    cut lem : (forall b1 b2,
-      proj AdvGate.Adv.g{1}.[(b1, b2)] = proj AdvGate.Adv.g{1}.[(b1, b2)]).
-    trivial.
-    trivial.
-    trivial.
-
-call
-  ((!Dkc.Dkc.b{1} = Dkc.Dkc.b{2}))
-  (!res{1} = res{2}).
-  fun.
-  skip.
-  trivial.
-intros resultDkc_L resultDkc_R.
-while (true).
-  wp.
-  call (true) (res{1} = res{2}).
-    admit.
-  admit.
-  wp.
-  app 1 1 : (true).
-    call (true) (true).
-      fun.
-      rnd.
-      skip.
-      trivial.
-    intros result_L0 result_R0.
-    skip.
-    trivial.
-    admit. (*Call adv*)
-admit. (*
-call
-  (true)
-  (res{1} = res{2}).
-  fun.
-  skip.
-  trivial.*)
-save.*)
-
-(*
-lemma MiddleEq2 :
-  forall (Adv <: Gate.Adv),
-    equiv [
-      Dkc.Game(Dkc.Dkc, AdvGate.Adv(Adv)).work ~ Dkc.Game(Dkc.Dkc, AdvGate.Adv(Adv)).work :
-      (! Dkc.Dkc.b{1}) /\ (AdvGate.Adv.l{1}=1) /\ (Dkc.Dkc.b{2}) /\ (AdvGate.Adv.l{2}=2) ==> res{1} = res{2}
-    ]
-proof.
-intros Adv.
-fun.
-inline {1} Dkc.Dkc.preInit.
-inline {1} Dkc.Dkc.get_challenge.
-inline {1} Dkc.Dkc.initialize.
-inline {1} AdvGate.Adv.gen_queries.
-inline {1} AdvGate.Adv.get_challenge.
-inline {2} Dkc.Dkc.preInit.
-inline {2} Dkc.Dkc.get_challenge.
-inline {2} Dkc.Dkc.initialize.
-inline {2} AdvGate.Adv.gen_queries.
-inline {2} AdvGate.Adv.get_challenge.
-wp.
-call (answer{1}=answer{2}) (res{1}=res{2}).
-admit.
-intros L R.
-wp.
-    rcondf {1} 8.
-    intros &m.
-    wp.
-
-app 17 17 : (realChallenge{1}=realChallenge{2} /\ AdvGate.Adv.l{1}=1 /\ AdvGate.Adv.l{2}=2/\AdvGate.Adv.input{1}=AdvGate.Adv.input{2}).
-  admit.
-  app 2 3 : (realChallenge{1}=realChallenge{2} /\ AdvGate.Adv.l{1}=1 /\ AdvGate.Adv.l{2}=2/\AdvGate.Adv.g{1}=AdvGate.Adv.g{2}/\AdvGate.Adv.input{1}=AdvGate.Adv.input{2}).
-    rcondf {1} 1;[intros &m;skip;trivial|].
-    rcondt {1} 1;[intros &m;skip;trivial|].
-    rcondf {2} 1;[intros &m;skip;trivial|].
-    rcondf {2} 1;[intros &m;skip;trivial|].
-    rcondt {2} 1;[intros &m;skip;trivial|].
-    call (AdvGate.Adv.input{1}=AdvGate.Adv.input{2}) (AdvGate.Adv.g{1}=AdvGate.Adv.g{2}/\AdvGate.Adv.input{1}=AdvGate.Adv.input{2}).
-      fun.
-      admit.
-    intros L2 R2.
-    skip.
-    trivial.
-  rcondf {1} 1;[intros &m;skip;trivial|].
-  skip;intros _ _ _;split;trivial.
-save.
-*)
-
-(*
-lemma fakeEq :
-  forall (Adv <: Gate.Adv),
-    equiv [
-      Dkc.Game(Dkc.Dkc, AdvGate.Adv(Adv)).work ~ RandBit.main :
-      AdvGate.Adv.l{1}=1 ==> res{1} = res{2}
-    ]
-proof.
-intros Adv.
-fun.
-inline {1} Dkc.Dkc.preInit.
-inline {1} Dkc.Dkc.get_challenge.
-inline {1} Dkc.Dkc.initialize.
-
-swap {1} 1 6.
-swap {1} 9 -2.
-wp.
-(*Call magical function*)
-save.*)
-
-(*
 lemma real :
-  forall &mDkc,(*forced b to 1 and l to 0*)
+  forall &mDkc,
     forall &mGate,
       forall (Adv <: Gate.Adv),
         Pr[Dkc.Game(Dkc.Dkc, AdvGate.Adv(Adv)).main()@ &mDkc:(*b /\ l=0 /\*) res] =
@@ -287,8 +23,8 @@ admit.
 save.
 
 lemma middle :
-  forall &mDkc1,(*forced b to 0 and l to 0*)
-    forall &mDkc2,(*forced b to 1 and l to 1*)
+  forall &mDkc1,
+    forall &mDkc2,
       forall (Adv <: Gate.Adv),
         Pr[Dkc.Game(Dkc.Dkc, AdvGate.Adv(Adv)).main()@ &mDkc1: !res] =
         Pr[Dkc.Game(Dkc.Dkc, AdvGate.Adv(Adv)).main()@ &mDkc2:  res]
@@ -296,30 +32,8 @@ proof.
 admit.
 save.
 
-module RandBit = {
-  fun main() : bool = {
-    var b : bool;
-    b = $Dbool.dbool;
-    return b;
-  }
-}.
-axiom RandBit : forall &m,
-      Pr[RandBit.main()@ &m:res] = 1%r / 2%r.
-
-lemma fakeEq :
-  forall (Adv <: Gate.Adv),
-    equiv [
-      Dkc.Game(Dkc.Dkc, AdvGate.Adv(Adv)).work ~ RandBit.main :
-      (! Dkc.Dkc.b) /\ (AdvGate.Adv.l=1) ==> res{1} = res{2}
-    ]
-proof.
-intros Adv.
-fun.
-admit.
-save.
-
 lemma fake :
-  forall &m,(*forced b to 0 and l to 1*)
+  forall &m,
   forall (Adv <: Gate.Adv),
       Pr[Dkc.Game(Dkc.Dkc, AdvGate.Adv(Adv)).main()@ &m: (!Dkc.Dkc.b)/\(*(AdvGate.Adv.l=1)/\*)(!res)] = 1%r / 2%r
 proof.
@@ -370,7 +84,18 @@ lemma DKCGateRelation2 :
       Pr[Gate.Game(Gate.PrvInd, Adv).main()@ &mGAR:res] <=
         Pr[Dkc.Game(Dkc.Dkc, AdvGate.Adv(Adv)).main()@ &mDKC:res]
 proof.
-admit.
+intros &mDKC Adv &mGAR.
+cut intro : (
+let a = Pr[Dkc.Game(Dkc.Dkc, AdvGate.Adv(Adv)).main()@ &mDKC:res] in
+let b = Pr[Gate.Game(Gate.PrvInd, Adv).main()@ &mGAR:res] in
+a <= b).
+intros a b.
+cut lem : (2%r * a - 1%r = (2%r * b - 1%r ) / 6%r);
+  [apply (DkcGateRelation1 &mDKC (<:Adv) &mGAR)|].
+cut lem2 : (a = b / 6%r + 5%r / 12%r). trivial.
+trivial.
+trivial.
+trivial.
 save.
 
 lemma PrvIndGarble :
@@ -380,8 +105,9 @@ lemma PrvIndGarble :
 proof.
 intros epsilon Adv &m.
 intros epPos.
-cut trans : (forall (a b c : real), a <= b => b <= c => a <= c);[trivial|].
-(*apply (trans Pr[Gate.Game(Gate.PrvInd, Adv).main()@ &m:res] Pr[Dkc.Game(Dkc.Dkc, AdvGate.Adv(Adv)).main()@ &m:res] epsilon _ _).*)
-apply (DKCGateRelation2 &m (<:Adv) &m  Pr[Gate.Game(Gate.PrvInd, Adv).main()@ &m:res] Pr[Dkc.Game(Dkc.Dkc, AdvGate.Adv(Adv)).main()@ &m:res]).
-admit.
+cut trans : (forall (a b c : real), a <= b => b < c => a <= c);[trivial|].
+apply (trans Pr[Gate.Game(Gate.PrvInd, Adv).main()@ &m:res] Pr[Dkc.Game(Dkc.Dkc, AdvGate.Adv(Adv)).main()@ &m:res] epsilon _ _).
+apply (DKCGateRelation2 &m (<:Adv) &m).
+apply (Dkc.DKCSec epsilon (<:AdvGate.Adv(Adv)) &m _).
+trivial.
 save.
